checker/element.v
@@ -3,6 +3,7 @@ Require Import Bool.
 Require Import List.
 Require Import prim.
 Require Import bounds.
+Require Import domain.
 
 (* Element constraint:
  * element x i [y_1, ..., y_n] <-> x = y_i.
@@ -12,40 +13,80 @@ Inductive element : Type :=
   | Elem : ivar -> ivar -> list Z -> element.
 
 (* This is kind of an awkward definition. *)
-Fixpoint eval_element_rec x i ys k theta :=
+Fixpoint eval_element_rec x i ys theta :=
   match ys with
   | nil => False
-  | cons y ys' =>
+  | cons (k, y) ys' =>
     (eval_ivar i theta = k /\ eval_ivar x theta = y)
-      \/ eval_element_rec x i ys' (k+1) theta
+      \/ eval_element_rec x i ys' theta
   end.
+
+Fixpoint augment_rec (A : Type) (xs : list A) (k : Z) :=
+  match xs with
+  | nil => nil
+  | (cons x xs') => cons (k, x) (augment_rec A xs' (k+1))
+  end.
+Definition augment (A : Type) (xs : list A) :=
+  augment_rec A xs 0.
 
 Definition eval_element (con : element) (theta : asg) :=
   match con with
-  | Elem x i ys => eval_element_rec x i ys 0 theta
+  | Elem x i ys => eval_element_rec x i (augment Z ys) theta
   end.
 
-Fixpoint check_element_rec x i ys k cl :=
+Fixpoint check_element_rec x i ys cl :=
   match ys with
   | nil => true
-  | cons y ys' =>
+  | cons (k, y) ys' =>
     negb
-      (inbounds_negcl cl i k && inbounds_negcl cl x y)
-      && check_element_rec x i ys' (k+1) cl
+      ((satb_dom (dom_from_negclause i cl) k)
+        && (satb_dom (dom_from_negclause x cl) y))
+      && check_element_rec x i ys' cl
   end.
 Definition check_element elem cl :=
   match elem with
-  | Elem x i ys => check_element_rec x i ys 0 cl
+  | Elem x i ys => check_element_rec x i (augment Z ys) cl
   end.
 
 (*
-Theorem check_element_rec_valid :
+Theorem check_element_valid :
+  forall (elem : element) (cl : clause) (theta : asg),
+    check_element elem cl = true ->
+      eval_element elem theta -> eval_clause cl theta.
+Proof.
+  unfold eval_element, check_element. destruct elem.
+  generalize (augment Z l).
+  intros l0 cl theta; induction l0.
+  unfold eval_element_rec; tauto.
+
+  unfold check_element_rec, eval_element_rec;
+    fold check_element_rec; fold eval_element_rec.
+  destruct a; simpl.
+  rewrite andb_true_iff, negb_true_iff, andb_false_iff.
+  intros.
+  destruct H as [ Hf Hrec ].
+  apply IHl0. exact Hrec.
+  destruct H0.
+*)
+(*
+Theorem check_element_valid :
   forall (elt : element) (cl : clause),
   check_element elt cl = true ->
     implies (eval_element elt) (eval_clause cl).
 Proof.
-  unfold implies; destruct elt; intros.
-  induction l.
+  unfold implies, check_element, eval_element.
+  intros elt cl; destruct elt.
+  intros; induction l.
+    unfold eval_element_rec in H0.
+    tauto.
+
+    unfold check_element_rec in H; fold check_element_rec in H.
+    unfold eval_element_rec in H0; fold eval_element_rec in H0.
+    apply andb_true_iff in H; destruct H as [Ha Hr].
+    rewrite negb_true_iff in Ha.
+    rewrite andb_false_iff in Ha.
+    destruct H as apply andb_true_iff in H.
+
 Qed.
    
 *)
